Refactoring and fixes to concurrent queue
but verif_queue_ex is now broken due to compspecs incompatibility.

progs/conc_queue.h
@@ -1,6 +1,7 @@
 struct queue_t;
 typedef struct queue_t queue_t;
 
+void *surely_malloc(size_t n);
 queue_t *q_new(void);
 void q_del(queue_t *tgt);
 void q_add(queue_t *tgt, void *e);
